\begin{problem}{M4}
Consider the two row operations 
\(R_2-4R_1\to R_2\) and \(\frac{1}{3}R_2\to R_2\)
showing \(A\sim B\):
\begin{align*}
A
  =
\begin{bmatrix}
1&2&3\\
4&5&6\\
7&8&9
\end{bmatrix}
  &\sim
\begin{bmatrix}
1&2&3\\
4-4(1)&5-4(2)&6-4(3)\\
7&8&9
\end{bmatrix}
  =
\begin{bmatrix}
1&2&3\\
0&-3&-6\\
7&8&9
\end{bmatrix}
  \\&\sim
\begin{bmatrix}
1&2&3\\
-\frac{1}{3}(0)&-\frac{1}{3}(-3)&-\frac{1}{3}(-6)\\
7&8&9
\end{bmatrix}
  =
\begin{bmatrix}
1&2&3\\
0&1&2\\
7&8&9
\end{bmatrix}
  = 
B
\end{align*}
Express these row operations as matrix multiplication
by writing \(B=QPA\) for two matrices \(Q,P\).
\end{problem}
\begin{solution}
\[
B
  =
\begin{bmatrix}
  1&0&0\\
  0&\frac{1}{3}&0\\
  0&0&1
\end{bmatrix}
\begin{bmatrix}
  1&0&0\\
  -4&1&0\\
  0&0&1
\end{bmatrix}
A
\]
\end{solution}


\begin{problem}{M4}
Consider the two row operations 
\(R_1\leftrightarrow R_2\) and \(R_3+R_1\to R_3\)
showing \(A\sim B\):
\begin{align*}
A
  =
\begin{bmatrix}
0&3&-1\\
1&2&3\\
-1&4&5
\end{bmatrix}
  &\sim
\begin{bmatrix}
1&2&3\\
0&3&-1\\
-1&4&5
\end{bmatrix}
  \\&\sim
\begin{bmatrix}
1&2&3\\
0&3&-1\\
-1+1&4+2&5+3
\end{bmatrix}
  =
\begin{bmatrix}
1&2&3\\
0&3&-1\\
0&6&8
\end{bmatrix}
  = 
B
\end{align*}
Express these row operations as matrix multiplication
by writing \(B=QPA\) for two matrices \(Q,P\).
\end{problem}
\begin{solution}
\[
B
  =
\begin{bmatrix}
  1&0&0\\
  0&1&0\\
  1&0&1
\end{bmatrix}
\begin{bmatrix}
  0&1&0\\
  1&0&0\\
  0&0&1
\end{bmatrix}
A
\]
\end{solution}


\begin{problem}{M4}
Consider the two row operations 
\(\frac{1}{2} R_3\to R_3\) and \(R_1\leftrightarrow R_3\)
showing \(A\sim B\):
\begin{align*}
A
  =
\begin{bmatrix}
-3&4&0\\
-7&2&3\\
2&-8&6
\end{bmatrix}
  &\sim
\begin{bmatrix}
-3&4&0\\
-7&2&3\\
\frac{1}{2}(2)&\frac{1}{2}(-8)&\frac{1}{2}(6)
\end{bmatrix}
  =
\begin{bmatrix}
-3&4&0\\
-7&2&3\\
1&-4&3
\end{bmatrix}
  \\&\sim
\begin{bmatrix}
1&-4&3\\
-7&2&3\\
-3&4&0
\end{bmatrix}
  =
B
\end{align*}
Express these row operations as matrix multiplication
by writing \(B=QPA\) for two matrices \(Q,P\).
\end{problem}
\begin{solution}
\[
B
  =
\begin{bmatrix}
  0&0&1\\
  0&1&0\\
  1&0&0
\end{bmatrix}
\begin{bmatrix}
  1&0&0\\
  0&1&0\\
  0&0&\frac{1}{2}
\end{bmatrix}
A
\]
\end{solution}
